pour commencer plus vite

plop.v
@@ -9,94 +9,40 @@ Variable rd : nat.
 
 Variable cmem :nat.
 
-Inductive op : Set :=
-| F : op
-| Fb : op
-| Wm  : op
-| Wd  : op
-| Rm  : op
-| Rd  : op
-| Dm  : op
-| Dd  : op.
+Inductive op_type : Set :=
+| F : op_type
+| Fb : op_type
+| Wm  : op_type
+| Wd  : op_type
+| Rm  : op_type
+| Rd  : op_type
+| Dm  : op_type
+| Dd  : op_type.
 
-Definition schedule := list (op * nat).
+Definition op := (op_type * nat)%type.
 
-Definition cost (o : op * nat) : nat :=
-  match o with
-    | (F,_) => uf
-    | (Fb,_) => ub
-    | (Wd,_) => wd
-    | (Rd,_) => rd
+Definition type (oi : op) :=
+  match oi with
+    | (o,i) => o
+  end.
+Definition index (oi : op) :=
+  match oi with
+    | (o,i) => i
+  end.
+
+Definition schedule := list op.
+
+Definition cost (o : op) : nat :=
+  match type o with
+    | F => uf
+    | Fb => ub
+    | Wd => wd
+    | Rd => rd
     | _ => 0
   end.
 
-SearchAbout fold_left.
-
 Definition cost_schedule (s : schedule) :=
   fold_left (fun c o => c + cost o) s 0.
-
-Definition memory := (list nat) %type.
-Definition disk := list nat.
-Definition buffer := nat.
-
-  
-Definition state := (buffer * buffer * memory * disk) %type.
-Definition get_top (e : state) :=
-  match e with (t,b,m,d) => t end.
-Definition get_bottom (e : state) :=
-  match e with (t,b,m,d) => b end.
-Definition get_memory (e : state) :=
-  match e with (t,b,m,d) => m end.
-Definition get_disk (e : state) :=
-  match e with (t,b,m,d) => d end.
-
-Definition size_memory e := length (get_memory e).
-
-Definition rmv := remove (eq_nat_dec).
-
-Definition eval e o i: state :=
-  match o with
-    | F => (i+1,get_bottom e,get_memory e,get_disk e)
-    | Fb => (i,i,get_memory e, get_disk e)
-    | Wm => (i,get_bottom e,i::(get_memory e),get_disk e)
-    | Wd => (i,get_bottom e,get_memory e,i::(get_disk e))
-    | Rm => (i,get_bottom e,get_memory e,get_disk e)
-    | Rd => (i,get_bottom e,get_memory e,get_disk e)
-    | Dm => (get_top e,get_bottom e,rmv i (get_memory e),get_disk e)
-    | Dd => (get_top e,get_bottom e,get_memory e,rmv i (get_disk e))
-  end.
-  
-Definition eval_schedule e s :=
-  fold_left (fun e' opi => match opi with (o,i) => eval e' o i end) s e.
-
-Inductive valid : state -> schedule -> Prop :=
-| vempty e s : s = nil -> valid e s
-| vf e i s : get_top e = i ->
-             valid (eval e F i) s ->
-             valid e ((F,i)::s)
-| vfb e i s : get_top e = i -> get_bottom e = i+1 ->
-              valid (eval e Fb i) s ->
-              valid e ((Fb,i)::s)
-| vwm e i s : get_top e = i -> size_memory e < cmem (* \/ In i (get_memory e) *) ->
-              valid (eval e Wm i) s ->
-              valid e ((Wm,i)::s)
-| vwd e i s : get_top e = i ->
-              valid (eval e Wd i) s ->
-              valid e ((Wd,i)::s)
-| vrm e i s : In i (get_memory e) ->
-              valid (eval e Rm i) s ->
-              valid e ((Rm,i)::s)
-| vrd e i s : In i (get_disk e) ->
-              valid (eval e Rd i) s ->
-              valid e ((Rd,i)::s)
-| vdm e i s : In i (get_memory e)->
-              valid (eval e Dm i) s ->
-              valid e ((Dm,i)::s)
-| vdd e i s : In i (get_disk e) ->
-              valid (eval e Dd i) s ->
-              valid e ((Dd,i)::s).
-
-Hint Constructors valid.
 
 Definition optimal s := forall s', cost_schedule s <= cost_schedule s'.
 
@@ -108,33 +54,115 @@ Proof.
   | apply h1].
 Qed.
 
-Lemma valid_app e s1 s2 : valid e (s1 ++ s2) <-> valid e s1 /\ valid (eval_schedule e s1) s2.
-Proof.
-  split;intro h.
-  induction s1.
-  split; auto.
-  inversion h.
-  rewrite<- app_comm_cons in H; inversion H.
-  SearchAbout (_::(_++_) = (_ ::_) ++ _).
-  destruct h.
+Definition memory := (list nat) %type.
+Definition disk := list nat.
+Definition buffer := nat.
+Definition state := (buffer * buffer * memory * disk) %type.
+Definition get_top (e : state) :=
+  match e with (t,b,m,d) => t end.
+Definition get_bottom (e : state) :=
+  match e with (t,b,m,d) => b end.
+Definition get_memory (e : state) :=
+  match e with (t,b,m,d) => m end.
+Definition get_disk (e : state) :=
+  match e with (t,b,m,d) => d end.
 
+Definition same_elts {A} l m :=
+  forall a : A, In a l <-> In a m.
+
+Definition equiv e f :=
+  get_top e = get_top f
+  /\ get_bottom e = get_bottom f
+  /\ same_elts (get_memory e) (get_memory f)
+  /\ same_elts (get_disk e) (get_disk f).
+
+Notation "e ≡ f" := (equiv e f) (at level 20). 
+
+Definition size_memory e := length (get_memory e).
+
+Definition rmv := remove (eq_nat_dec).
+
+Definition eval_op e o : state :=
+  let i := index o in
+  match type o with
+    | F => (i+1,get_bottom e,get_memory e,get_disk e)
+    | Fb => (i,i,get_memory e, get_disk e)
+    | Wm => (i,get_bottom e,i::(get_memory e),get_disk e)
+    | Wd => (i,get_bottom e,get_memory e,i::(get_disk e))
+    | Rm => (i,get_bottom e,get_memory e,get_disk e)
+    | Rd => (i,get_bottom e,get_memory e,get_disk e)
+    | Dm => (get_top e,get_bottom e,rmv i (get_memory e),get_disk e)
+    | Dd => (get_top e,get_bottom e,get_memory e,rmv i (get_disk e))
+  end.
   
-Lemma no_double_write_mem e s i :
-  forall s1 s2 s3,
-  s = s1 ++ ((Wm,i)::nil) ++ s2 ++ ((Wm,i)::nil) ++ s3 ->
-  valid e s -> optimal s ->
-  ~ In (Dm,i) s2  ->
-  exists s', s' = s1 ++ ((Wm,i)::nil) ++ s2 ++ s3
-             /\ valid e s'
-             /\ optimal s'.
+Definition eval_schedule e s :=
+  fold_left eval_op s e.
+
+Definition valid_op e o : Prop :=
+  let i := index o in
+  match type o with
+    | F => get_top e = i
+    | Fb => get_top e = i /\ get_bottom e = i+1
+    | Wm => get_top e = i /\ size_memory e < cmem
+    | Wd => get_top e = i
+    | Rm => In i (get_memory e)
+    | Rd => In i (get_disk e)
+    | Dm => In i (get_memory e)
+    | Dd => In i (get_disk e)
+  end.
+
+Inductive valid_schedule : state -> schedule -> Prop :=
+| vempty e s : s = nil -> valid_schedule e s
+| vcons e o s : valid_op e o -> valid_schedule (eval_op e o) s ->
+                valid_schedule e (o::s).
+
+Hint Constructors valid_schedule.
+
+
+Lemma valid_app e s1 s2 :
+  valid_schedule e (s1 ++ s2) <->
+  valid_schedule e s1 /\ valid_schedule (eval_schedule e s1) s2.
 Proof.
-intros s1 s2 s3 h1 h2 h3 h4.
-exists (s1 ++ ((Wm, i) :: nil) ++ s2 ++ s3); repeat split; auto.
+Admitted.
 
+Notation "[ a , b ]" := ((a,b)::nil) (at level 50).
 
-Lemma no_super_write_mem e s i :
-  valid e s -> optimal s -> In i (get_memory e) ->
-  exists s1 s2, s = s1 ++ ((Wm,i)::nil) ++ s2 ->
-                   exists s', s' = s1 ++ s2
-                              /\ valid e s'
-                              /\ optimal s'.
+Definition no_double_write_mem_i s (i : nat) :=
+  ~ (exists s1 s2 s3, s = s1 ++ [Wm,i] ++ s2 ++ [Wm,i] ++ s3
+                      /\ ~ In (Dm,i) s2).
+
+Fixpoint remove_write_mem_i s (i : nat) :=
+  match s with
+    | nil => nil
+    | (Dm,j)::s => if beq_nat i j
+                   then (Dm,j)::s
+                   else (Dm,j)::(remove_write_mem_i s i)
+    | (Wm,j)::s => if beq_nat i j
+                   then remove_write_mem_i s i
+                   else (Wm,j)::(remove_write_mem_i s i)
+    | oi::s => oi::(remove_write_mem_i s i)
+  end.
+    
+Fixpoint remove_double_write_mem s :=
+  match s with
+    | nil => nil
+    | (Wm,i)::s =>
+      (Wm,i)::(remove_write_mem_i (remove_double_write_mem s) i)
+    | oi::s => oi::(remove_double_write_mem s)
+  end.
+
+Lemma correct_rdwm s e :
+  eval_schedule e s ≡ eval_schedule e (remove_double_write_mem s).
+Admitted.
+Lemma valid_rdwm s e :
+  valid_schedule e s ->
+  valid_schedule e (remove_double_write_mem s).
+Admitted.
+Lemma optimal_rdwm s e :
+  valid_schedule e s ->
+  valid_schedule e (remove_double_write_mem s).
+Admitted.
+Lemma no_dwm_rdwm s :
+  forall i,
+    no_double_write_mem_i (remove_double_write_mem s) i. 
+Admitted.
